rewrite manifest to play well with mpl test-vectors

TestVectors/runtimes/java/src/main/java/software/amazon/cryptography/encryptionsdk/internaldafny/wrapped/__default.java
@@ -20,9 +20,10 @@ public class __default extends _ExternBase___default {
       throw new IllegalArgumentException("Native AWS Encryption SDK for Java does not support NetV4_0_0_RetryPolicy.ALLOW_RETRY");
     }
     CommitmentPolicy commitmentPolicy = _esdkDafnyCommitmentPolicyToNative(wrappedConfig.commitmentPolicy());
+    int maxEncryptedDataKeys = wrappedConfig.maxEncryptedDataKeys() == 0 ? 1 : (int) wrappedConfig.maxEncryptedDataKeys();
     final AwsCrypto awsCrypto = AwsCrypto.builder()
       .withCommitmentPolicy(commitmentPolicy)
-      .withMaxEncryptedDataKeys((int) wrappedConfig.maxEncryptedDataKeys())
+      .withMaxEncryptedDataKeys(maxEncryptedDataKeys)
       .build();
     TestESDK wrappedEsdk = TestESDK.builder().impl(awsCrypto).build();
     return software.amazon.cryptography.encryptionsdk.internaldafny._ExternBase___default.CreateSuccessOfClient(wrappedEsdk);
