TestVectors/dafny/ESDK/src/LibraryIndex.dfy
@@ -28,4 +28,16 @@ module
       netV4_0_0_RetryPolicy := None
     )
   }
+  function method WrappedAwsEncryptionSdkConfig(
+    commitmentPolicy: AwsCryptographyMaterialProvidersTypes.ESDKCommitmentPolicy,
+    maxEncryptedDataKeys: CountingNumbers,
+    netV4_0_0_RetryPolicy: NetV4_0_0_RetryPolicy
+  ) : AwsEncryptionSdkConfig
+  {
+    AwsEncryptionSdkConfig(
+      commitmentPolicy := Some(commitmentPolicy),
+      maxEncryptedDataKeys := Some(maxEncryptedDataKeys),
+      netV4_0_0_RetryPolicy := Some(netV4_0_0_RetryPolicy)
+    )
+  }
 }
